process syntax updated

processes/process.sig
@@ -6,7 +6,7 @@
   prod: Functor
 
   psend     : process
-  pssend    : lpart -> "prod" ("prod" (llabel, expr), process) -> process
+  pssend    : lpart -> llabel -> expr -> process -> process
   psreceive : lpart -> "list" ("prod" ("prod" (llabel, expr), process)) -> process
   psite     : expr -> process -> process -> process
   psmu      : (process -> process) -> process
