processes/process.v
@@ -1,35 +1,49 @@
 Require Import ST.processes.unscoped.
 (* From mathcomp Require Import all_ssreflect. *)
 From Paco Require Import paco.
-Require Import String List (*ZArith*).
+Require Import String List ZArith.
 Local Open Scope string_scope.
 Import ListNotations.
 
 Notation participant := string.
 Notation label := string.
 
+Inductive value: Type :=
+ | vint : Z    -> value
+ | vbool: bool -> value
+ | vunit: unit -> value.
+
 Inductive expr: Type :=
-  | ebool: bool   -> expr
-  | enat : nat    -> expr
-(*   | eint : Z      -> expr *)
-  | eunit: unit   -> expr
+  | eval : value  -> expr
   | evar : string -> expr
+  | esucc: expr   -> expr
   | einv : expr   -> expr
-(*   | eisgt: expr   -> expr *)
+  | eneg : expr   -> expr
+  | eisgt: expr   -> expr
   | eistt: expr   -> expr.
 
+Inductive mqueue: Type := 
+  | nilq: mqueue
+  | mesq: participant -> label -> value -> mqueue -> mqueue.
+
+Fixpoint conq (m1 m2: mqueue): mqueue :=
+  match m1 with
+    | nilq         => m2
+    | mesq p l v q => mesq p l v (conq q m2)
+  end.
+
 Inductive process  : Type :=
-  | ps_var    : nat -> process 
+  | ps_var    : fin -> process 
   | ps_end    : process 
-  | ps_send   : participant -> (label*expr*process) -> process 
-  | ps_receive: participant -> list (label*expr*process) -> process 
+  | ps_send   : participant -> label -> expr -> process -> process 
+  | ps_receive: participant -> list(label*expr*process) -> process 
   | ps_ite    : expr -> process -> process -> process 
   | ps_mu     : process -> process.
 
-Lemma congr_ps_end  : ps_end  = ps_end  .
+Lemma congr_ps_end  : ps_end  = ps_end.
 Proof. congruence. Qed.
 
-Lemma congr_ps_send  { s0 : participant   } { s1 : prod (prod (label  ) (expr  )) (process  ) } { t0 : participant   } { t1 : prod (prod (label  ) (expr  )) (process  ) } (H1 : s0 = t0) (H2 : s1 = t1) : ps_send  s0 s1 = ps_send  t0 t1 .
+Lemma congr_ps_send  { s0 : participant   } { s1 : label   } { s2 : expr   } { s3 : process   } { t0 : participant   } { t1 : label   } { t2 : expr   } { t3 : process   } (H1 : s0 = t0) (H2 : s1 = t1) (H3 : s2 = t2) (H4 : s3 = t3) : ps_send  s0 s1 s2 s3 = ps_send  t0 t1 t2 t3 .
 Proof. congruence. Qed.
 
 Lemma congr_ps_receive  { s0 : participant   } { s1 : list (prod (prod (label  ) (expr  )) (process  )) } { t0 : participant   } { t1 : list (prod (prod (label  ) (expr  )) (process  )) } (H1 : s0 = t0) (H2 : s1 = t1) : ps_receive  s0 s1 = ps_receive  t0 t1 .
@@ -41,158 +55,158 @@ Proof. congruence. Qed.
 Lemma congr_ps_mu  { s0 : process   } { t0 : process   } (H1 : s0 = t0) : ps_mu  s0 = ps_mu  t0 .
 Proof. congruence. Qed.
 
-Definition upRen_process_process   (xi : ( nat ) -> nat) : ( nat ) -> nat :=
+Definition upRen_process_process   (xi : ( fin ) -> fin) : ( fin ) -> fin :=
   (up_ren) xi.
 
-Fixpoint ren_process   (xiprocess : ( nat ) -> nat) (s : process ) : process  :=
+Fixpoint ren_process   (xiprocess : ( fin ) -> fin) (s : process ) : process  :=
     match s return process  with
     | ps_var  s => (ps_var ) (xiprocess s)
     | ps_end   => ps_end 
-    | ps_send  s0 s1 => ps_send  ((fun x => x) s0) ((prod_map (prod_map (fun x => x) (fun x => x)) (ren_process xiprocess)) s1)
+    | ps_send  s0 s1 s2 s3 => ps_send  ((fun x => x) s0) ((fun x => x) s1) ((fun x => x) s2) ((ren_process xiprocess) s3)
     | ps_receive  s0 s1 => ps_receive  ((fun x => x) s0) ((list_map (prod_map (prod_map (fun x => x) (fun x => x)) (ren_process xiprocess))) s1)
     | ps_ite  s0 s1 s2 => ps_ite  ((fun x => x) s0) ((ren_process xiprocess) s1) ((ren_process xiprocess) s2)
     | ps_mu  s0 => ps_mu  ((ren_process (upRen_process_process xiprocess)) s0)
     end.
 
-Definition up_process_process   (sigma : ( nat ) -> process ) : ( nat ) -> process  :=
-  (scons) ((ps_var ) (var_zero)) ((funcomp) (ren_process (shift)) sigma).
+Definition up_process_process   (sigma : ( fin ) -> process ) : ( fin ) -> process  :=
+  (scons) ((ps_var ) (var_zero)) ((funcomp) (ren_process (unscoped.shift)) sigma).
 
-Fixpoint subst_process   (sigmaprocess : ( nat ) -> process ) (s : process ) : process  :=
+Fixpoint subst_process   (sigmaprocess : ( fin ) -> process ) (s : process ) : process  :=
     match s return process  with
     | ps_var  s => sigmaprocess s
     | ps_end   => ps_end 
-    | ps_send  s0 s1 => ps_send  ((fun x => x) s0) ((prod_map (prod_map (fun x => x) (fun x => x)) (subst_process sigmaprocess)) s1)
+    | ps_send  s0 s1 s2 s3 => ps_send  ((fun x => x) s0) ((fun x => x) s1) ((fun x => x) s2) ((subst_process sigmaprocess) s3)
     | ps_receive  s0 s1 => ps_receive  ((fun x => x) s0) ((list_map (prod_map (prod_map (fun x => x) (fun x => x)) (subst_process sigmaprocess))) s1)
     | ps_ite  s0 s1 s2 => ps_ite  ((fun x => x) s0) ((subst_process sigmaprocess) s1) ((subst_process sigmaprocess) s2)
     | ps_mu  s0 => ps_mu  ((subst_process (up_process_process sigmaprocess)) s0)
     end.
 
-Definition upId_process_process  (sigma : ( nat ) -> process ) (Eq : forall x, sigma x = (ps_var ) x) : forall x, (up_process_process sigma) x = (ps_var ) x :=
+Definition upId_process_process  (sigma : ( fin ) -> process ) (Eq : forall x, sigma x = (ps_var ) x) : forall x, (up_process_process sigma) x = (ps_var ) x :=
   fun n => match n with
-  | S nat_n => (ap) (ren_process (shift)) (Eq nat_n)
+  | S fin_n => (ap) (ren_process (unscoped.shift)) (Eq fin_n)
   | 0  => eq_refl
   end.
 
-Fixpoint idSubst_process  (sigmaprocess : ( nat ) -> process ) (Eqprocess : forall x, sigmaprocess x = (ps_var ) x) (s : process ) : subst_process sigmaprocess s = s :=
+Fixpoint idSubst_process  (sigmaprocess : ( fin ) -> process ) (Eqprocess : forall x, sigmaprocess x = (ps_var ) x) (s : process ) : subst_process sigmaprocess s = s :=
     match s return subst_process sigmaprocess s = s with
     | ps_var  s => Eqprocess s
     | ps_end   => congr_ps_end 
-    | ps_send  s0 s1 => congr_ps_send ((fun x => (eq_refl) x) s0) ((prod_id (prod_id (fun x => (eq_refl) x) (fun x => (eq_refl) x)) (idSubst_process sigmaprocess Eqprocess)) s1)
+    | ps_send  s0 s1 s2 s3 => congr_ps_send ((fun x => (eq_refl) x) s0) ((fun x => (eq_refl) x) s1) ((fun x => (eq_refl) x) s2) ((idSubst_process sigmaprocess Eqprocess) s3)
     | ps_receive  s0 s1 => congr_ps_receive ((fun x => (eq_refl) x) s0) ((list_id (prod_id (prod_id (fun x => (eq_refl) x) (fun x => (eq_refl) x)) (idSubst_process sigmaprocess Eqprocess))) s1)
     | ps_ite  s0 s1 s2 => congr_ps_ite ((fun x => (eq_refl) x) s0) ((idSubst_process sigmaprocess Eqprocess) s1) ((idSubst_process sigmaprocess Eqprocess) s2)
     | ps_mu  s0 => congr_ps_mu ((idSubst_process (up_process_process sigmaprocess) (upId_process_process (_) Eqprocess)) s0)
     end.
 
-Definition upExtRen_process_process   (xi : ( nat ) -> nat) (zeta : ( nat ) -> nat) (Eq : forall x, xi x = zeta x) : forall x, (upRen_process_process xi) x = (upRen_process_process zeta) x :=
+Definition upExtRen_process_process   (xi : ( fin ) -> fin) (zeta : ( fin ) -> fin) (Eq : forall x, xi x = zeta x) : forall x, (upRen_process_process xi) x = (upRen_process_process zeta) x :=
   fun n => match n with
-  | S nat_n => (ap) (shift) (Eq nat_n)
+  | S fin_n => (ap) (unscoped.shift) (Eq fin_n)
   | 0  => eq_refl
   end.
 
-Fixpoint extRen_process   (xiprocess : ( nat ) -> nat) (zetaprocess : ( nat ) -> nat) (Eqprocess : forall x, xiprocess x = zetaprocess x) (s : process ) : ren_process xiprocess s = ren_process zetaprocess s :=
+Fixpoint extRen_process   (xiprocess : ( fin ) -> fin) (zetaprocess : ( fin ) -> fin) (Eqprocess : forall x, xiprocess x = zetaprocess x) (s : process ) : ren_process xiprocess s = ren_process zetaprocess s :=
     match s return ren_process xiprocess s = ren_process zetaprocess s with
     | ps_var  s => (ap) (ps_var ) (Eqprocess s)
     | ps_end   => congr_ps_end 
-    | ps_send  s0 s1 => congr_ps_send ((fun x => (eq_refl) x) s0) ((prod_ext (prod_ext (fun x => (eq_refl) x) (fun x => (eq_refl) x)) (extRen_process xiprocess zetaprocess Eqprocess)) s1)
+    | ps_send  s0 s1 s2 s3 => congr_ps_send ((fun x => (eq_refl) x) s0) ((fun x => (eq_refl) x) s1) ((fun x => (eq_refl) x) s2) ((extRen_process xiprocess zetaprocess Eqprocess) s3)
     | ps_receive  s0 s1 => congr_ps_receive ((fun x => (eq_refl) x) s0) ((list_ext (prod_ext (prod_ext (fun x => (eq_refl) x) (fun x => (eq_refl) x)) (extRen_process xiprocess zetaprocess Eqprocess))) s1)
     | ps_ite  s0 s1 s2 => congr_ps_ite ((fun x => (eq_refl) x) s0) ((extRen_process xiprocess zetaprocess Eqprocess) s1) ((extRen_process xiprocess zetaprocess Eqprocess) s2)
     | ps_mu  s0 => congr_ps_mu ((extRen_process (upRen_process_process xiprocess) (upRen_process_process zetaprocess) (upExtRen_process_process (_) (_) Eqprocess)) s0)
     end.
 
-Definition upExt_process_process   (sigma : ( nat ) -> process ) (tau : ( nat ) -> process ) (Eq : forall x, sigma x = tau x) : forall x, (up_process_process sigma) x = (up_process_process tau) x :=
+Definition upExt_process_process   (sigma : ( fin ) -> process ) (tau : ( fin ) -> process ) (Eq : forall x, sigma x = tau x) : forall x, (up_process_process sigma) x = (up_process_process tau) x :=
   fun n => match n with
-  | S nat_n => (ap) (ren_process (shift)) (Eq nat_n)
+  | S fin_n => (ap) (ren_process (unscoped.shift)) (Eq fin_n)
   | 0  => eq_refl
   end.
 
-Fixpoint ext_process   (sigmaprocess : ( nat ) -> process ) (tauprocess : ( nat ) -> process ) (Eqprocess : forall x, sigmaprocess x = tauprocess x) (s : process ) : subst_process sigmaprocess s = subst_process tauprocess s :=
+Fixpoint ext_process   (sigmaprocess : ( fin ) -> process ) (tauprocess : ( fin ) -> process ) (Eqprocess : forall x, sigmaprocess x = tauprocess x) (s : process ) : subst_process sigmaprocess s = subst_process tauprocess s :=
     match s return subst_process sigmaprocess s = subst_process tauprocess s with
     | ps_var  s => Eqprocess s
     | ps_end   => congr_ps_end 
-    | ps_send  s0 s1 => congr_ps_send ((fun x => (eq_refl) x) s0) ((prod_ext (prod_ext (fun x => (eq_refl) x) (fun x => (eq_refl) x)) (ext_process sigmaprocess tauprocess Eqprocess)) s1)
+    | ps_send  s0 s1 s2 s3 => congr_ps_send ((fun x => (eq_refl) x) s0) ((fun x => (eq_refl) x) s1) ((fun x => (eq_refl) x) s2) ((ext_process sigmaprocess tauprocess Eqprocess) s3)
     | ps_receive  s0 s1 => congr_ps_receive ((fun x => (eq_refl) x) s0) ((list_ext (prod_ext (prod_ext (fun x => (eq_refl) x) (fun x => (eq_refl) x)) (ext_process sigmaprocess tauprocess Eqprocess))) s1)
     | ps_ite  s0 s1 s2 => congr_ps_ite ((fun x => (eq_refl) x) s0) ((ext_process sigmaprocess tauprocess Eqprocess) s1) ((ext_process sigmaprocess tauprocess Eqprocess) s2)
     | ps_mu  s0 => congr_ps_mu ((ext_process (up_process_process sigmaprocess) (up_process_process tauprocess) (upExt_process_process (_) (_) Eqprocess)) s0)
     end.
 
-Definition up_ren_ren_process_process    (xi : ( nat ) -> nat) (tau : ( nat ) -> nat) (theta : ( nat ) -> nat) (Eq : forall x, ((funcomp) tau xi) x = theta x) : forall x, ((funcomp) (upRen_process_process tau) (upRen_process_process xi)) x = (upRen_process_process theta) x :=
+Definition up_ren_ren_process_process    (xi : ( fin ) -> fin) (tau : ( fin ) -> fin) (theta : ( fin ) -> fin) (Eq : forall x, ((funcomp) tau xi) x = theta x) : forall x, ((funcomp) (upRen_process_process tau) (upRen_process_process xi)) x = (upRen_process_process theta) x :=
   up_ren_ren xi tau theta Eq.
 
-Fixpoint compRenRen_process    (xiprocess : ( nat ) -> nat) (zetaprocess : ( nat ) -> nat) (rhoprocess : ( nat ) -> nat) (Eqprocess : forall x, ((funcomp) zetaprocess xiprocess) x = rhoprocess x) (s : process ) : ren_process zetaprocess (ren_process xiprocess s) = ren_process rhoprocess s :=
+Fixpoint compRenRen_process    (xiprocess : ( fin ) -> fin) (zetaprocess : ( fin ) -> fin) (rhoprocess : ( fin ) -> fin) (Eqprocess : forall x, ((funcomp) zetaprocess xiprocess) x = rhoprocess x) (s : process ) : ren_process zetaprocess (ren_process xiprocess s) = ren_process rhoprocess s :=
     match s return ren_process zetaprocess (ren_process xiprocess s) = ren_process rhoprocess s with
     | ps_var  s => (ap) (ps_var ) (Eqprocess s)
     | ps_end   => congr_ps_end 
-    | ps_send  s0 s1 => congr_ps_send ((fun x => (eq_refl) x) s0) ((prod_comp (prod_comp (fun x => (eq_refl) x) (fun x => (eq_refl) x)) (compRenRen_process xiprocess zetaprocess rhoprocess Eqprocess)) s1)
+    | ps_send  s0 s1 s2 s3 => congr_ps_send ((fun x => (eq_refl) x) s0) ((fun x => (eq_refl) x) s1) ((fun x => (eq_refl) x) s2) ((compRenRen_process xiprocess zetaprocess rhoprocess Eqprocess) s3)
     | ps_receive  s0 s1 => congr_ps_receive ((fun x => (eq_refl) x) s0) ((list_comp (prod_comp (prod_comp (fun x => (eq_refl) x) (fun x => (eq_refl) x)) (compRenRen_process xiprocess zetaprocess rhoprocess Eqprocess))) s1)
     | ps_ite  s0 s1 s2 => congr_ps_ite ((fun x => (eq_refl) x) s0) ((compRenRen_process xiprocess zetaprocess rhoprocess Eqprocess) s1) ((compRenRen_process xiprocess zetaprocess rhoprocess Eqprocess) s2)
     | ps_mu  s0 => congr_ps_mu ((compRenRen_process (upRen_process_process xiprocess) (upRen_process_process zetaprocess) (upRen_process_process rhoprocess) (up_ren_ren (_) (_) (_) Eqprocess)) s0)
     end.
 
-Definition up_ren_subst_process_process    (xi : ( nat ) -> nat) (tau : ( nat ) -> process ) (theta : ( nat ) -> process ) (Eq : forall x, ((funcomp) tau xi) x = theta x) : forall x, ((funcomp) (up_process_process tau) (upRen_process_process xi)) x = (up_process_process theta) x :=
+Definition up_ren_subst_process_process    (xi : ( fin ) -> fin) (tau : ( fin ) -> process ) (theta : ( fin ) -> process ) (Eq : forall x, ((funcomp) tau xi) x = theta x) : forall x, ((funcomp) (up_process_process tau) (upRen_process_process xi)) x = (up_process_process theta) x :=
   fun n => match n with
-  | S nat_n => (ap) (ren_process (shift)) (Eq nat_n)
+  | S fin_n => (ap) (ren_process (unscoped.shift)) (Eq fin_n)
   | 0  => eq_refl
   end.
 
-Fixpoint compRenSubst_process    (xiprocess : ( nat ) -> nat) (tauprocess : ( nat ) -> process ) (thetaprocess : ( nat ) -> process ) (Eqprocess : forall x, ((funcomp) tauprocess xiprocess) x = thetaprocess x) (s : process ) : subst_process tauprocess (ren_process xiprocess s) = subst_process thetaprocess s :=
+Fixpoint compRenSubst_process    (xiprocess : ( fin ) -> fin) (tauprocess : ( fin ) -> process ) (thetaprocess : ( fin ) -> process ) (Eqprocess : forall x, ((funcomp) tauprocess xiprocess) x = thetaprocess x) (s : process ) : subst_process tauprocess (ren_process xiprocess s) = subst_process thetaprocess s :=
     match s return subst_process tauprocess (ren_process xiprocess s) = subst_process thetaprocess s with
     | ps_var  s => Eqprocess s
     | ps_end   => congr_ps_end 
-    | ps_send  s0 s1 => congr_ps_send ((fun x => (eq_refl) x) s0) ((prod_comp (prod_comp (fun x => (eq_refl) x) (fun x => (eq_refl) x)) (compRenSubst_process xiprocess tauprocess thetaprocess Eqprocess)) s1)
+    | ps_send  s0 s1 s2 s3 => congr_ps_send ((fun x => (eq_refl) x) s0) ((fun x => (eq_refl) x) s1) ((fun x => (eq_refl) x) s2) ((compRenSubst_process xiprocess tauprocess thetaprocess Eqprocess) s3)
     | ps_receive  s0 s1 => congr_ps_receive ((fun x => (eq_refl) x) s0) ((list_comp (prod_comp (prod_comp (fun x => (eq_refl) x) (fun x => (eq_refl) x)) (compRenSubst_process xiprocess tauprocess thetaprocess Eqprocess))) s1)
     | ps_ite  s0 s1 s2 => congr_ps_ite ((fun x => (eq_refl) x) s0) ((compRenSubst_process xiprocess tauprocess thetaprocess Eqprocess) s1) ((compRenSubst_process xiprocess tauprocess thetaprocess Eqprocess) s2)
     | ps_mu  s0 => congr_ps_mu ((compRenSubst_process (upRen_process_process xiprocess) (up_process_process tauprocess) (up_process_process thetaprocess) (up_ren_subst_process_process (_) (_) (_) Eqprocess)) s0)
     end.
 
-Definition up_subst_ren_process_process    (sigma : ( nat ) -> process ) (zetaprocess : ( nat ) -> nat) (theta : ( nat ) -> process ) (Eq : forall x, ((funcomp) (ren_process zetaprocess) sigma) x = theta x) : forall x, ((funcomp) (ren_process (upRen_process_process zetaprocess)) (up_process_process sigma)) x = (up_process_process theta) x :=
+Definition up_subst_ren_process_process    (sigma : ( fin ) -> process ) (zetaprocess : ( fin ) -> fin) (theta : ( fin ) -> process ) (Eq : forall x, ((funcomp) (ren_process zetaprocess) sigma) x = theta x) : forall x, ((funcomp) (ren_process (upRen_process_process zetaprocess)) (up_process_process sigma)) x = (up_process_process theta) x :=
   fun n => match n with
-  | S nat_n => (eq_trans) (compRenRen_process (shift) (upRen_process_process zetaprocess) ((funcomp) (shift) zetaprocess) (fun x => eq_refl) (sigma nat_n)) ((eq_trans) ((eq_sym) (compRenRen_process zetaprocess (shift) ((funcomp) (shift) zetaprocess) (fun x => eq_refl) (sigma nat_n))) ((ap) (ren_process (shift)) (Eq nat_n)))
+  | S fin_n => (eq_trans) (compRenRen_process (unscoped.shift) (upRen_process_process zetaprocess) ((funcomp) (unscoped.shift) zetaprocess) (fun x => eq_refl) (sigma fin_n)) ((eq_trans) ((eq_sym) (compRenRen_process zetaprocess (unscoped.shift) ((funcomp) (unscoped.shift) zetaprocess) (fun x => eq_refl) (sigma fin_n))) ((ap) (ren_process (unscoped.shift)) (Eq fin_n)))
   | 0  => eq_refl
   end.
 
-Fixpoint compSubstRen_process    (sigmaprocess : ( nat ) -> process ) (zetaprocess : ( nat ) -> nat) (thetaprocess : ( nat ) -> process ) (Eqprocess : forall x, ((funcomp) (ren_process zetaprocess) sigmaprocess) x = thetaprocess x) (s : process ) : ren_process zetaprocess (subst_process sigmaprocess s) = subst_process thetaprocess s :=
+Fixpoint compSubstRen_process    (sigmaprocess : ( fin ) -> process ) (zetaprocess : ( fin ) -> fin) (thetaprocess : ( fin ) -> process ) (Eqprocess : forall x, ((funcomp) (ren_process zetaprocess) sigmaprocess) x = thetaprocess x) (s : process ) : ren_process zetaprocess (subst_process sigmaprocess s) = subst_process thetaprocess s :=
     match s return ren_process zetaprocess (subst_process sigmaprocess s) = subst_process thetaprocess s with
     | ps_var  s => Eqprocess s
     | ps_end   => congr_ps_end 
-    | ps_send  s0 s1 => congr_ps_send ((fun x => (eq_refl) x) s0) ((prod_comp (prod_comp (fun x => (eq_refl) x) (fun x => (eq_refl) x)) (compSubstRen_process sigmaprocess zetaprocess thetaprocess Eqprocess)) s1)
+    | ps_send  s0 s1 s2 s3 => congr_ps_send ((fun x => (eq_refl) x) s0) ((fun x => (eq_refl) x) s1) ((fun x => (eq_refl) x) s2) ((compSubstRen_process sigmaprocess zetaprocess thetaprocess Eqprocess) s3)
     | ps_receive  s0 s1 => congr_ps_receive ((fun x => (eq_refl) x) s0) ((list_comp (prod_comp (prod_comp (fun x => (eq_refl) x) (fun x => (eq_refl) x)) (compSubstRen_process sigmaprocess zetaprocess thetaprocess Eqprocess))) s1)
     | ps_ite  s0 s1 s2 => congr_ps_ite ((fun x => (eq_refl) x) s0) ((compSubstRen_process sigmaprocess zetaprocess thetaprocess Eqprocess) s1) ((compSubstRen_process sigmaprocess zetaprocess thetaprocess Eqprocess) s2)
     | ps_mu  s0 => congr_ps_mu ((compSubstRen_process (up_process_process sigmaprocess) (upRen_process_process zetaprocess) (up_process_process thetaprocess) (up_subst_ren_process_process (_) (_) (_) Eqprocess)) s0)
     end.
 
-Definition up_subst_subst_process_process    (sigma : ( nat ) -> process ) (tauprocess : ( nat ) -> process ) (theta : ( nat ) -> process ) (Eq : forall x, ((funcomp) (subst_process tauprocess) sigma) x = theta x) : forall x, ((funcomp) (subst_process (up_process_process tauprocess)) (up_process_process sigma)) x = (up_process_process theta) x :=
+Definition up_subst_subst_process_process    (sigma : ( fin ) -> process ) (tauprocess : ( fin ) -> process ) (theta : ( fin ) -> process ) (Eq : forall x, ((funcomp) (subst_process tauprocess) sigma) x = theta x) : forall x, ((funcomp) (subst_process (up_process_process tauprocess)) (up_process_process sigma)) x = (up_process_process theta) x :=
   fun n => match n with
-  | S nat_n => (eq_trans) (compRenSubst_process (shift) (up_process_process tauprocess) ((funcomp) (up_process_process tauprocess) (shift)) (fun x => eq_refl) (sigma nat_n)) ((eq_trans) ((eq_sym) (compSubstRen_process tauprocess (shift) ((funcomp) (ren_process (shift)) tauprocess) (fun x => eq_refl) (sigma nat_n))) ((ap) (ren_process (shift)) (Eq nat_n)))
+  | S fin_n => (eq_trans) (compRenSubst_process (unscoped.shift) (up_process_process tauprocess) ((funcomp) (up_process_process tauprocess) (unscoped.shift)) (fun x => eq_refl) (sigma fin_n)) ((eq_trans) ((eq_sym) (compSubstRen_process tauprocess (unscoped.shift) ((funcomp) (ren_process (unscoped.shift)) tauprocess) (fun x => eq_refl) (sigma fin_n))) ((ap) (ren_process (unscoped.shift)) (Eq fin_n)))
   | 0  => eq_refl
   end.
 
-Fixpoint compSubstSubst_process    (sigmaprocess : ( nat ) -> process ) (tauprocess : ( nat ) -> process ) (thetaprocess : ( nat ) -> process ) (Eqprocess : forall x, ((funcomp) (subst_process tauprocess) sigmaprocess) x = thetaprocess x) (s : process ) : subst_process tauprocess (subst_process sigmaprocess s) = subst_process thetaprocess s :=
+Fixpoint compSubstSubst_process    (sigmaprocess : ( fin ) -> process ) (tauprocess : ( fin ) -> process ) (thetaprocess : ( fin ) -> process ) (Eqprocess : forall x, ((funcomp) (subst_process tauprocess) sigmaprocess) x = thetaprocess x) (s : process ) : subst_process tauprocess (subst_process sigmaprocess s) = subst_process thetaprocess s :=
     match s return subst_process tauprocess (subst_process sigmaprocess s) = subst_process thetaprocess s with
     | ps_var  s => Eqprocess s
     | ps_end   => congr_ps_end 
-    | ps_send  s0 s1 => congr_ps_send ((fun x => (eq_refl) x) s0) ((prod_comp (prod_comp (fun x => (eq_refl) x) (fun x => (eq_refl) x)) (compSubstSubst_process sigmaprocess tauprocess thetaprocess Eqprocess)) s1)
+    | ps_send  s0 s1 s2 s3 => congr_ps_send ((fun x => (eq_refl) x) s0) ((fun x => (eq_refl) x) s1) ((fun x => (eq_refl) x) s2) ((compSubstSubst_process sigmaprocess tauprocess thetaprocess Eqprocess) s3)
     | ps_receive  s0 s1 => congr_ps_receive ((fun x => (eq_refl) x) s0) ((list_comp (prod_comp (prod_comp (fun x => (eq_refl) x) (fun x => (eq_refl) x)) (compSubstSubst_process sigmaprocess tauprocess thetaprocess Eqprocess))) s1)
     | ps_ite  s0 s1 s2 => congr_ps_ite ((fun x => (eq_refl) x) s0) ((compSubstSubst_process sigmaprocess tauprocess thetaprocess Eqprocess) s1) ((compSubstSubst_process sigmaprocess tauprocess thetaprocess Eqprocess) s2)
     | ps_mu  s0 => congr_ps_mu ((compSubstSubst_process (up_process_process sigmaprocess) (up_process_process tauprocess) (up_process_process thetaprocess) (up_subst_subst_process_process (_) (_) (_) Eqprocess)) s0)
     end.
 
-Definition rinstInst_up_process_process   (xi : ( nat ) -> nat) (sigma : ( nat ) -> process ) (Eq : forall x, ((funcomp) (ps_var ) xi) x = sigma x) : forall x, ((funcomp) (ps_var ) (upRen_process_process xi)) x = (up_process_process sigma) x :=
+Definition rinstInst_up_process_process   (xi : ( fin ) -> fin) (sigma : ( fin ) -> process ) (Eq : forall x, ((funcomp) (ps_var ) xi) x = sigma x) : forall x, ((funcomp) (ps_var ) (upRen_process_process xi)) x = (up_process_process sigma) x :=
   fun n => match n with
-  | S nat_n => (ap) (ren_process (shift)) (Eq nat_n)
+  | S fin_n => (ap) (ren_process (unscoped.shift)) (Eq fin_n)
   | 0  => eq_refl
   end.
 
-Fixpoint rinst_inst_process   (xiprocess : ( nat ) -> nat) (sigmaprocess : ( nat ) -> process ) (Eqprocess : forall x, ((funcomp) (ps_var ) xiprocess) x = sigmaprocess x) (s : process ) : ren_process xiprocess s = subst_process sigmaprocess s :=
+Fixpoint rinst_inst_process   (xiprocess : ( fin ) -> fin) (sigmaprocess : ( fin ) -> process ) (Eqprocess : forall x, ((funcomp) (ps_var ) xiprocess) x = sigmaprocess x) (s : process ) : ren_process xiprocess s = subst_process sigmaprocess s :=
     match s return ren_process xiprocess s = subst_process sigmaprocess s with
     | ps_var  s => Eqprocess s
     | ps_end   => congr_ps_end 
-    | ps_send  s0 s1 => congr_ps_send ((fun x => (eq_refl) x) s0) ((prod_ext (prod_ext (fun x => (eq_refl) x) (fun x => (eq_refl) x)) (rinst_inst_process xiprocess sigmaprocess Eqprocess)) s1)
+    | ps_send  s0 s1 s2 s3 => congr_ps_send ((fun x => (eq_refl) x) s0) ((fun x => (eq_refl) x) s1) ((fun x => (eq_refl) x) s2) ((rinst_inst_process xiprocess sigmaprocess Eqprocess) s3)
     | ps_receive  s0 s1 => congr_ps_receive ((fun x => (eq_refl) x) s0) ((list_ext (prod_ext (prod_ext (fun x => (eq_refl) x) (fun x => (eq_refl) x)) (rinst_inst_process xiprocess sigmaprocess Eqprocess))) s1)
     | ps_ite  s0 s1 s2 => congr_ps_ite ((fun x => (eq_refl) x) s0) ((rinst_inst_process xiprocess sigmaprocess Eqprocess) s1) ((rinst_inst_process xiprocess sigmaprocess Eqprocess) s2)
     | ps_mu  s0 => congr_ps_mu ((rinst_inst_process (upRen_process_process xiprocess) (up_process_process sigmaprocess) (rinstInst_up_process_process (_) (_) Eqprocess)) s0)
     end.
 
-Lemma rinstInst_process   (xiprocess : ( nat ) -> nat) : ren_process xiprocess = subst_process ((funcomp) (ps_var ) xiprocess) .
+Lemma rinstInst_process   (xiprocess : ( fin ) -> fin) : ren_process xiprocess = subst_process ((funcomp) (ps_var ) xiprocess) .
 Proof. exact ((FunctionalExtensionality.functional_extensionality _ _ ) (fun x => rinst_inst_process xiprocess (_) (fun n => eq_refl) x)). Qed.
 
 Lemma instId_process  : subst_process (ps_var ) = id .
@@ -201,42 +215,42 @@ Proof. exact ((FunctionalExtensionality.functional_extensionality _ _ ) (fun x =
 Lemma rinstId_process  : @ren_process   (id) = id .
 Proof. exact ((eq_trans) (rinstInst_process ((id) (_))) instId_process). Qed.
 
-Lemma varL_process   (sigmaprocess : ( nat ) -> process ) : (funcomp) (subst_process sigmaprocess) (ps_var ) = sigmaprocess .
+Lemma varL_process   (sigmaprocess : ( fin ) -> process ) : (funcomp) (subst_process sigmaprocess) (ps_var ) = sigmaprocess .
 Proof. exact ((FunctionalExtensionality.functional_extensionality _ _ ) (fun x => eq_refl)). Qed.
 
-Lemma varLRen_process   (xiprocess : ( nat ) -> nat) : (funcomp) (ren_process xiprocess) (ps_var ) = (funcomp) (ps_var ) xiprocess .
+Lemma varLRen_process   (xiprocess : ( fin ) -> fin) : (funcomp) (ren_process xiprocess) (ps_var ) = (funcomp) (ps_var ) xiprocess .
 Proof. exact ((FunctionalExtensionality.functional_extensionality _ _ ) (fun x => eq_refl)). Qed.
 
-Lemma compComp_process    (sigmaprocess : ( nat ) -> process ) (tauprocess : ( nat ) -> process ) (s : process ) : subst_process tauprocess (subst_process sigmaprocess s) = subst_process ((funcomp) (subst_process tauprocess) sigmaprocess) s .
+Lemma compComp_process    (sigmaprocess : ( fin ) -> process ) (tauprocess : ( fin ) -> process ) (s : process ) : subst_process tauprocess (subst_process sigmaprocess s) = subst_process ((funcomp) (subst_process tauprocess) sigmaprocess) s .
 Proof. exact (compSubstSubst_process sigmaprocess tauprocess (_) (fun n => eq_refl) s). Qed.
 
-Lemma compComp'_process    (sigmaprocess : ( nat ) -> process ) (tauprocess : ( nat ) -> process ) : (funcomp) (subst_process tauprocess) (subst_process sigmaprocess) = subst_process ((funcomp) (subst_process tauprocess) sigmaprocess) .
+Lemma compComp'_process    (sigmaprocess : ( fin ) -> process ) (tauprocess : ( fin ) -> process ) : (funcomp) (subst_process tauprocess) (subst_process sigmaprocess) = subst_process ((funcomp) (subst_process tauprocess) sigmaprocess) .
 Proof. exact ((FunctionalExtensionality.functional_extensionality _ _ ) (fun n => compComp_process sigmaprocess tauprocess n)). Qed.
 
-Lemma compRen_process    (sigmaprocess : ( nat ) -> process ) (zetaprocess : ( nat ) -> nat) (s : process ) : ren_process zetaprocess (subst_process sigmaprocess s) = subst_process ((funcomp) (ren_process zetaprocess) sigmaprocess) s .
+Lemma compRen_process    (sigmaprocess : ( fin ) -> process ) (zetaprocess : ( fin ) -> fin) (s : process ) : ren_process zetaprocess (subst_process sigmaprocess s) = subst_process ((funcomp) (ren_process zetaprocess) sigmaprocess) s .
 Proof. exact (compSubstRen_process sigmaprocess zetaprocess (_) (fun n => eq_refl) s). Qed.
 
-Lemma compRen'_process    (sigmaprocess : ( nat ) -> process ) (zetaprocess : ( nat ) -> nat) : (funcomp) (ren_process zetaprocess) (subst_process sigmaprocess) = subst_process ((funcomp) (ren_process zetaprocess) sigmaprocess) .
+Lemma compRen'_process    (sigmaprocess : ( fin ) -> process ) (zetaprocess : ( fin ) -> fin) : (funcomp) (ren_process zetaprocess) (subst_process sigmaprocess) = subst_process ((funcomp) (ren_process zetaprocess) sigmaprocess) .
 Proof. exact ((FunctionalExtensionality.functional_extensionality _ _ ) (fun n => compRen_process sigmaprocess zetaprocess n)). Qed.
 
-Lemma renComp_process    (xiprocess : ( nat ) -> nat) (tauprocess : ( nat ) -> process ) (s : process ) : subst_process tauprocess (ren_process xiprocess s) = subst_process ((funcomp) tauprocess xiprocess) s .
+Lemma renComp_process    (xiprocess : ( fin ) -> fin) (tauprocess : ( fin ) -> process ) (s : process ) : subst_process tauprocess (ren_process xiprocess s) = subst_process ((funcomp) tauprocess xiprocess) s .
 Proof. exact (compRenSubst_process xiprocess tauprocess (_) (fun n => eq_refl) s). Qed.
 
-Lemma renComp'_process    (xiprocess : ( nat ) -> nat) (tauprocess : ( nat ) -> process ) : (funcomp) (subst_process tauprocess) (ren_process xiprocess) = subst_process ((funcomp) tauprocess xiprocess) .
+Lemma renComp'_process    (xiprocess : ( fin ) -> fin) (tauprocess : ( fin ) -> process ) : (funcomp) (subst_process tauprocess) (ren_process xiprocess) = subst_process ((funcomp) tauprocess xiprocess) .
 Proof. exact ((FunctionalExtensionality.functional_extensionality _ _ ) (fun n => renComp_process xiprocess tauprocess n)). Qed.
 
-Lemma renRen_process    (xiprocess : ( nat ) -> nat) (zetaprocess : ( nat ) -> nat) (s : process ) : ren_process zetaprocess (ren_process xiprocess s) = ren_process ((funcomp) zetaprocess xiprocess) s .
+Lemma renRen_process    (xiprocess : ( fin ) -> fin) (zetaprocess : ( fin ) -> fin) (s : process ) : ren_process zetaprocess (ren_process xiprocess s) = ren_process ((funcomp) zetaprocess xiprocess) s .
 Proof. exact (compRenRen_process xiprocess zetaprocess (_) (fun n => eq_refl) s). Qed.
 
-Lemma renRen'_process    (xiprocess : ( nat ) -> nat) (zetaprocess : ( nat ) -> nat) : (funcomp) (ren_process zetaprocess) (ren_process xiprocess) = ren_process ((funcomp) zetaprocess xiprocess) .
+Lemma renRen'_process    (xiprocess : ( fin ) -> fin) (zetaprocess : ( fin ) -> fin) : (funcomp) (ren_process zetaprocess) (ren_process xiprocess) = ren_process ((funcomp) zetaprocess xiprocess) .
 Proof. exact ((FunctionalExtensionality.functional_extensionality _ _ ) (fun n => renRen_process xiprocess zetaprocess n)). Qed.
 
 
-Global Instance Subst_process   : Subst1 (( nat ) -> process ) (process ) (process ) := @subst_process   .
+Global Instance Subst_process   : Subst1 (( fin ) -> process ) (process ) (process ) := @subst_process   .
 
-Global Instance Ren_process   : Ren1 (( nat ) -> nat) (process ) (process ) := @ren_process   .
+Global Instance Ren_process   : Ren1 (( fin ) -> fin) (process ) (process ) := @ren_process   .
 
-Global Instance VarInstance_process  : Var (nat) (process ) := @ps_var  .
+Global Instance VarInstance_process  : Var (fin) (process ) := @ps_var  .
 
 Notation "x '__process'" := (ps_var x) (at level 5, format "x __process") : subst_scope.
 
